\documentclass{article}
\usepackage{preamble}

\begin{document}
    Interventions:
    \begin{align*}
        M(i,j) & = \s{M_{k,l}|\forall l ,\forall s_k.  e_j \in \mathcal{E} \amp \s{e_i,e_j} \subseteq s_k} \\
        E(i,j) & = \s{E_{k,l}|\forall l ,\forall s_k.  e_j \in \mathcal{E} \amp \s{e_i,e_j} \subseteq s_k} \\
        ( \s{x_1,x_2,...,x_n} = y ) 
        & =  (x_1 = y \amp x_2 = y \amp ... \amp x_n = y) \\
    \end{align*}

    \begin{align*}
        C_{i,j} \leftarrow true 
        & \Rightarrow M(i,j) = false, E(i,j) = false  \\
        M_{k,i} \leftarrow true
        & \Rightarrow \s{M_{k',i}|\forall k'. s_{k'} \subset s_k \text{ or } s_k \subset s_{k'}} = false \\
        & \phantom{\Rightarrow} 
        \s{E_{k',i}| \forall k'. s_k \subseteq s_{k'} \amp Con(E_{k',i}) } = true \\
        E_{k,i} \leftarrow true 
        & \Rightarrow \s{E_{k',i}| \forall k'. s_k \subseteq s_{k'} \amp Con(E_{k',i}) } = true \\
        C_{i,j} \leftarrow false
        & \Rightarrow 
    \end{align*}
\end{document}