\begin{frame}{Composing Causality}
    \begin{align*}
        \mathrm{E}                   & = (E,\#,\vdash)                          \\
        \mathcal{M}                  & = \mathfrak{M}(\mathrm{E}),s \subseteq E \\
        \varphi                      & = X_1 = x_1 \wedge X_2 = x_2
        \wedge ... \wedge X_n = x_n                                             \\
        \mathcal{M},\varphi \vDash s & \iff \varphi \text{ Cause }
        s \in \mathcal{F}(\mathrm{E})
    \end{align*}
    \begin{itemize}
        \item $\mathrm{E}_0 = (E_0,\#_0,\vdash_0)$, $\mathrm{E}_1 = (E_1,\#_1,\vdash_1)$
        \item $\mathrm{E} = (E,\#,\vdash) = \mathrm{E}_0 + \mathrm{E}_1$
    \end{itemize}
    \begin{align*}
        \iota_k(e)          & = (k,e)                     \\
        \iota_k(X)          & = \s{\iota_{k}(e)| e \in s} \\
        \mathcal{M},\varphi & \vDash s \iff               \\
                            & \left(
        \exists s_0 \subseteq E_0. s = \iota_0(s_0)
        ,\exists \varphi_0 \in \mathcal{M}_0. \iota_0(\varphi_0) = \varphi.
        \mathcal{M}_0,\varphi_0 \vDash s_0
        \right)                                           \\
                            & \vee \left(
        \exists s_1 \subseteq E_1. s = \iota_1(s_1)
        ,\exists \varphi_1 \in \mathcal{M}_1. \iota_1(\varphi_1) = \varphi.
        \mathcal{M}_1,\varphi_1 \vDash s_1
        \right)
    \end{align*}
\end{frame}